Examples.lean
@@ -35,5 +35,6 @@ import Examples.RF_RP_Switching_alt
 import Examples.Regev
 import Examples.Schnorr
 import Examples.SchnorrExtractorRuntime
+import Examples.SealedSender.AspectObservation
 import Examples.Signature
 import Examples.SimpleTwoServerPIR
